GroupoidModel/Russell_PER_MS/Inversion.lean
@@ -97,13 +97,15 @@ theorem inv_all :
   case cong_lam' B _ _ _ _ _ _ _ _ _ _ _ _ =>
     refine ⟨?_, ?_, ?_, WfTm.conv (WfTm.lam' (B := B) ?_ ?_) ?_⟩
     all_goals grind [WfTm.lam', EqTp.cong_pi', EqTp.refl_tp, EqTp.symm_tp, WfTp.pi']
-  case cong_app' Γ ihB ihf iha =>
+  case cong_app' Aeq _ _ _aeq Γ ihA ihB ihf iha =>
     refine ⟨Γ, ?_, ?_,
       WfTm.conv
-        (WfTm.app' iha.2.1 ihB.2.2
+        (WfTm.app'
+          ihA.2.2
+          (tp_conv_binder Γ ihA.2.1 ihA.2.2 Aeq ihB.2.2)
           (WfTm.conv ihf.2.2.2 ?_)
-          iha.2.2.2)
-        ?_⟩
+          (WfTm.conv iha.2.2.2 Aeq))
+          ?_⟩
     all_goals grind [EqTp.cong_pi', EqTp.refl_tp, tp_inst, eqtp_inst, EqTp.symm_tp, WfTm.app']
   case cong_pair' ihB iht ihu =>
     refine ⟨?_, ?_, ?_,
@@ -289,7 +291,7 @@ theorem WfTm.lam {Γ A B t l l'} :
 theorem WfTm.app {Γ A B f a l l'} :
     Γ ⊢[max l l'] f : .pi l l' A B →
     Γ ⊢[l] a : A →
-    Γ ⊢[l'] .app l l' B f a : B.subst a.toSb :=
+    Γ ⊢[l'] .app l l' A B f a : B.subst a.toSb :=
   fun hf ha =>
     have ⟨_, hA, hB⟩ := hf.wf_tp.inv_pi
     WfTm.app' hA hB hf ha
@@ -321,12 +323,13 @@ theorem EqTm.cong_lam {Γ A A' B t t' l l'} :
     Γ ⊢[max l l'] .lam l l' A t ≡ .lam l l' A' t' : .pi l l' A B :=
   fun hAA' htt' => EqTm.cong_lam' hAA'.wf_left hAA'.wf_right hAA' htt'
 
-theorem EqTm.cong_app {Γ A B B' f f' a a' l l'} :
+theorem EqTm.cong_app {Γ A A' B B' f f' a a' l l'} :
+    Γ ⊢[l] A ≡ A' →
     (A, l) :: Γ ⊢[l'] B ≡ B' →
     Γ ⊢[max l l'] f ≡ f' : .pi l l' A B →
     Γ ⊢[l] a ≡ a' : A →
-    Γ ⊢[l'] .app l l' B f a ≡ .app l l' B' f' a' : B.subst a.toSb :=
-  fun hBB' hff' haa' => EqTm.cong_app' haa'.wf_tp hBB' hff' haa'
+    Γ ⊢[l'] .app l l' A B f a ≡ .app l l' A' B' f' a' : B.subst a.toSb :=
+  fun hAA' hBB' hff' haa' => EqTm.cong_app' hAA'.wf_left hAA' hBB' hff' haa'
 
 theorem EqTm.cong_pair {Γ A B B' t t' u u' l l'} :
     (A, l) :: Γ ⊢[l'] B ≡ B' →
@@ -352,7 +355,7 @@ theorem EqTm.cong_snd {Γ A A' B B' p p' l l'} :
 theorem EqTm.app_lam {Γ A B t u l l'} :
     (A, l) :: Γ ⊢[l'] t : B →
     Γ ⊢[l] u : A →
-    Γ ⊢[l'] .app l l' B (.lam l l' A t) u ≡ t.subst u.toSb : B.subst u.toSb :=
+    Γ ⊢[l'] .app l l' A B (.lam l l' A t) u ≡ t.subst u.toSb : B.subst u.toSb :=
   fun ht hu => EqTm.app_lam' hu.wf_tp ht.wf_tp ht hu
 
 theorem EqTm.fst_pair {Γ A B t u l l'} :
@@ -371,7 +374,7 @@ theorem EqTm.snd_pair {Γ A B t u l l'} :
 
 theorem EqTm.lam_app {Γ A B f l l'} :
     Γ ⊢[max l l'] f : .pi l l' A B →
-    Γ ⊢[max l l'] f ≡ .lam l l' A (.app l l' (B.subst (Expr.up Expr.wk)) (f.subst Expr.wk) (.bvar 0)) : .pi l l' A B :=
+    Γ ⊢[max l l'] f ≡ .lam l l' A (.app l l' (A.subst Expr.wk) (B.subst (Expr.up Expr.wk)) (f.subst Expr.wk) (.bvar 0)) : .pi l l' A B :=
   fun hf =>
     have ⟨_, hA, hB⟩ := hf.wf_tp.inv_pi
     EqTm.lam_app' hA hB hf
@@ -405,27 +408,23 @@ theorem WfTm.inv_bvar {Γ A i l} : Γ ⊢[l] .bvar i : A →
     grind [EqTp.refl_tp, EqTp.symm_tp, EqTp.trans_tp, WfCtx.lookup_wf]
 
 theorem WfTm.inv_lam {Γ A C b l₀ l l'} : Γ ⊢[l₀] .lam l l' A b : C →
-    l₀ = max l l' ∧ (Γ ⊢[l] A) ∧
-      ∃ B, ((A, l) :: Γ ⊢[l'] b : B) ∧ (Γ ⊢[max l l'] C ≡ .pi l l' A B) := by
+    l₀ = max l l' ∧ ∃ B,
+      ((A, l) :: Γ ⊢[l'] b : B) ∧ (Γ ⊢[max l l'] C ≡ .pi l l' A B) := by
   suffices
       ∀ {Γ l t C}, Γ ⊢[l] t : C → ∀ {A b l₁ l₂}, t = .lam l₁ l₂ A b →
-        l = max l₁ l₂ ∧ (Γ ⊢[l₁] A) ∧
-          ∃ B, ((A, l₁) :: Γ ⊢[l₂] b : B) ∧ (Γ ⊢[max l₁ l₂] C ≡ .pi l₁ l₂ A B) from
+        l = max l₁ l₂ ∧ ∃ B,
+          ((A, l₁) :: Γ ⊢[l₂] b : B) ∧ (Γ ⊢[max l₁ l₂] C ≡ .pi l₁ l₂ A B) from
     fun h => this h rfl
   mutual_induction WfCtx <;>
     grind [WfTp.pi, WfTm.wf_tp, EqTp.refl_tp, EqTp.symm_tp, EqTp.trans_tp]
 
-theorem WfTm.inv_app {Γ B C f a l l'} : Γ ⊢[l'] .app l l' B f a : C →
-    ∃ A,
-      (Γ ⊢[max l l'] f : .pi l l' A B) ∧
-      (Γ ⊢[l] a : A) ∧
+theorem WfTm.inv_app {Γ A B C f a l₀ l l'} : Γ ⊢[l₀] .app l l' A B f a : C →
+    l₀ = l' ∧ (Γ ⊢[max l l'] f : .pi l l' A B) ∧ (Γ ⊢[l] a : A) ∧
       (Γ ⊢[l'] C ≡ B.subst a.toSb) := by
   suffices
-      ∀ {Γ l t C}, Γ ⊢[l] t : C → ∀ {B f a l₁}, t = .app l₁ l B f a →
-        ∃ A,
-          (Γ ⊢[max l₁ l] f : .pi l₁ l A B) ∧
-          (Γ ⊢[l₁] a : A) ∧
-          (Γ ⊢[l] C ≡ B.subst a.toSb) from
+      ∀ {Γ l₀ t C}, Γ ⊢[l₀] t : C → ∀ {A B f a l l'}, t = .app l l' A B f a →
+        l₀ = l' ∧ (Γ ⊢[max l l'] f : .pi l l' A B) ∧ (Γ ⊢[l] a : A) ∧
+          (Γ ⊢[l'] C ≡ B.subst a.toSb) from
     fun h => this h rfl
   mutual_induction WfCtx <;>
     grind [InvProof.tp_inst, WfTp.wf_ctx, EqTp.refl_tp, EqTp.symm_tp, EqTp.trans_tp]
